theories/theories/utp_relations.thy
@@ -1,0 +1,35 @@
+(******************************************************************************)
+(* Project: Mechanisation of the UTP                                          *)
+(* File: utp_relations.thy                                                    *)
+(* Authors: Simon Foster, University of York                                  *)
+(******************************************************************************)
+
+header {* UTP Theory of Relations *}
+
+theory utp_relations
+imports 
+  utp_base
+begin
+
+subsection {* Relational Healthiness Condition *}
+
+definition RELH :: "'a WF_PREDICATE \<Rightarrow> 'a WF_PREDICATE" where
+"RELH(P) = (\<exists>\<^sub>p NON_REL_VAR. P)"
+
+lemma RELH_idem:
+  "RELH (RELH P) = RELH P"
+  by (simp add:RELH_def eval)
+
+lemma RELH_WF_RELATION [closure]:
+  "RELH P \<in> WF_RELATION"
+  by (simp add:RELH_def WF_RELATION_def unrest)
+
+lemma RELH_iff_WF_RELATION:
+  "P = RELH P \<longleftrightarrow> P \<in> WF_RELATION"
+  apply (rule)
+  apply (simp_all add:RELH_def WF_RELATION_def unrest)
+  apply (metis (full_types) UNREST_ExistsP_simple subset_refl)
+  apply (utp_pred_tac)
+done
+
+end
